Separate out a file on cells

Orderedtree/DOrderedTree/Internal/Model.lean
@@ -4,6 +4,7 @@ Released under Apache 2.0 license as described in the file LICENSE.
 Authors: Markus Himmel
 -/
 import Orderedtree.DOrderedTree.Internal.Impl
+import Orderedtree.DOrderedTree.Internal.Cell
 
 /-!
 # Model implementations of ordered tree functions
@@ -23,59 +24,6 @@ namespace Impl
 /-!
 ## General infrastructure
 -/
-
-/-- Type for representing the place in a binary search tree where a mapping for `k` could live. -/
-structure Cell (α : Type u) [Ord α] (β : α → Type v) (k : α) where
-  /-- The mapping. -/
-  inner : Option ((a : α) × β a)
-  /-- If there is a mapping, then it has a matching key. -/
-  property : ∀ [OrientedOrd α], ∀ p, inner = some p → compare k p.1 = .eq
-
-namespace Cell
-
-/-- Create a cell with a matching key. -/
-def ofEq [Ord α] {k : α} (k' : α) (v' : β k') (hcmp : ∀ [OrientedOrd α], compare k k' = .eq) :
-    Cell α β k :=
-  ⟨some ⟨k', v'⟩, by intro _ p hp; obtain rfl := Option.some_inj.1 hp; simpa using hcmp⟩
-
-/-- Create a cell with a matching key. -/
-def of [Ord α] (k : α) (v : β k) : Cell α β k :=
-  .ofEq k v (by intro; simp)
-
-@[simp] theorem ofEq_inner [Ord α] {k k' : α} {v' : β k'} {h} :
-  (Cell.ofEq k' v' h : Cell α β k).inner = some ⟨k', v'⟩ := rfl
-@[simp] theorem of_inner [Ord α] {k : α} {v : β k} : (Cell.of k v).inner = some ⟨k, v⟩ := rfl
-
-/-- Create an empty cell. -/
-def empty [Ord α] {k : α} : Cell α β k :=
-  ⟨none, by simp⟩
-
-@[simp] theorem empty_inner [Ord α] {k : α} : (Cell.empty : Cell α β k).inner = none := rfl
-
-def contains [Ord α] {k : α} (c : Cell α β k) : Bool :=
-  c.inner.isSome
-
-@[simp] theorem contains_of [Ord α] {k : α} {v : β k} : (Cell.of k v).contains = true := rfl
-@[simp] theorem contains_ofEq [Ord α] {k k' : α} {v' : β k'} {h} :
-    (Cell.ofEq k' v' h : Cell α β k).contains = true := rfl
-@[simp] theorem contains_empty [Ord α] {k : α} : (Cell.empty : Cell α β k).contains = false := rfl
-
-def get? [Ord α] [OrientedOrd α] [LawfulEqOrd α] {k : α} (c : Cell α β k) : Option (β k) :=
-  match h : c.inner with
-  | none => none
-  | some p => some (cast (congrArg β (eq_of_compare (c.property _ h)).symm) p.2)
-
-@[simp]
-theorem get?_empty [Ord α] [OrientedOrd α] [LawfulEqOrd α] {k : α} :
-    (Cell.empty : Cell α β k).get? = none :=
-  rfl
-
-def get [Ord α] [OrientedOrd α] [LawfulEqOrd α] {k : α} (c : Cell α β k) (h : c.contains) : β k :=
-  match hc : c.inner with
-  | none => False.elim (by simp [contains, hc] at h)
-  | some p => (cast (congrArg β (eq_of_compare (c.property _ hc)).symm) p.2)
-
-end Cell
 
 /-- General tree-traversal function. -/
 def applyPartition [Ord α] (k : α) (l : Impl α β)
